---
layout: page
---
### Claim
$$\Sigma;\alpha \vDash \beta \text{ iff }\Sigma\vDash(\alpha\to\beta)$$ 

### Proof
"$$\Rightarrow$$" 

For the forward direction, assume that $$\Sigma;\alpha\vDash\beta$$ 

Let $$v$$ be an arbitrary truth assignment which satisfies $$\Sigma$$ 

**Case 1: $$v$$ also satisfies $$\alpha$$**

In this case, since we already know that $$\Sigma;\alpha\vDash\beta$$, we know that the truth assignment $$v$$ will also satisfy $$\beta$$. Thus, $$\overline{v}(\alpha) = \overline{v}(\beta) =T$$ so that $$\overline{v}(\alpha\to\beta) = T$$

**Case 2: $$v$$ does not satisfy $$\alpha$$ 

In this case, $$\overline{v}(\alpha) = F$$, so no matter the value of $$\overline{v}(\beta)$$, $$\overline{v}(\alpha\to\beta) = T$$ 


Since $$v$$ is arbitrary in both cases, we see that that $$\Sigma\vDash(\alpha\to\beta)$$

"$$\Leftarrow$$"

For the backwards direction, assume that $$\Sigma\vDash(\alpha\to\beta)$$

Let $$v$$ be a truth assignment satisfying $$\Sigma;\alpha$$.
Then $$\overline{v}(\alpha)=T$$ and $$\overline{v}(\alpha\to\beta)=T$$, since $$\Sigma\vDash(\alpha\to\beta)$$ 
Suppose $$\overline{v}(\beta)=F$$, then since $$\overline{v}(\alpha)=T$$ and by the axioms which $$\overline{v}$$ must follow, it must be that $$\overline{v}(\alpha\to\beta) = F$$, which is a contradiction. Thus, we must have that $$\overline{v}(\beta) = T$$ 

Since $$v$$ was an arbitrary truth assignment satisfying $$\Sigma;\alpha$$, we have that $$\Sigma;\alpha\vDash\beta$$ 

###### Part (b)
Claim: $$\alpha$$ is tautologically equivalent to $$\beta$$ if and only if $$(\alpha\leftrightarrow\beta)$$ is a tautology.

"$$\Rightarrow$$"

For the forward direction, assume $$\alpha$$ and $$\beta$$ are tautologically equivalent.

Now, let $$v$$ be an arbitrary truth assignment. 

**Case 1: $$\overline{v}(\alpha) =F$$**
In this case, we must have that $$\overline{v}(\beta) = F$$, since $$\beta\vDash\alpha$$.

**Case 2: $$\overline{v}(\alpha)=T$$**
In this case, we must have that $$\overline{v}(\beta) = T$$, since $$\alpha\vDash\beta$$

Both cases show that for an arbitrary truth assignment $$v$$, it will be that $$\overline{v}(\alpha) = \overline{v}(\beta)$$.
Thus, $$(\alpha\leftrightarrow\beta)$$ will be true for any truth assignment, meaning it is a tautology.

"$$\Leftarrow$$"

Now for the backwards direction, we assume that $$(\alpha\leftrightarrow\beta)$$ is a tautology. 

Let $$v$$ be a truth assignment such that $$\overline{v}(\alpha)=T$$, then since $$\overline{v}(\alpha\leftrightarrow\beta) = T$$, we must have that $$\overline{v}(\beta) = T$$. Thus, $$\alpha\vDash\beta$$

Now, let $$v$$ be a truth assignment such that $$\overline{v}(\beta) =T$$. By the same logic as the preceding sentences, it must be that $$\overline{v}(\alpha) = T$$, so that $$\beta \vDash\alpha$$.

Therefore, $$\alpha$$ and $$\beta$$ are tautologically equivalent.
