---
layout: page
---
### Problem
Of the following three formulas, which tautologically imply which?
(a) $$(A\leftrightarrow B)$$
(b) $$(\lnot((A\to B)\to (\lnot(B\to A)))) = \alpha$$
(c) $$(((\lnot A)\lor B)\land (A\lor (\lnot B))) = \beta$$
### Solution
I claim that all three statements are tautologically equivalent, consider the following truth table
\begin{array}{|c|c|}
A & B & (\lnot A) & (\lnot B) & (A\to B) & (\lnot(B\to A)) & (A\leftrightarrow B) & \alpha & \beta \\
\hline
T & T & F & F & T & F & T & T & T\\
T & F & F & T & F & F & F & F & F\\
F & T & T & F & T & T & F & F & F\\
F & F & T & T & T & F & T & T & T\end{array}
Notice that an arbitrary truth assignment $$v$$ satisfies $$(A\leftrightarrow B)$$ if and only if it also satisfies $$\alpha=(\lnot((A\to B)\to (\lnot(B\to A))))$$ and $$\beta = (((\lnot A)\lor B)\land (A\lor (\lnot B)))$$. Similarly, $$v$$ satisfies $$\beta$$ if and only if it also satisfies $$(A\leftrightarrow B)$$ and $$\alpha$$, and $$v$$ satisfies $$\alpha$$ if and only if it also satisfies $$(A\leftrightarrow B)$$ and $$\beta$$. Thus, all three statements are tautologically equivalent.
