---
layout: page
---
### Problem
Show that neither of the following two formulas tautologically imply each other
\begin{gather}(A\leftrightarrow(B\leftrightarrow C))\\ ((A\land(B\land C))\lor((\lnot A)\land((\lnot B)\land (\lnot C))))\end{gather}
### Solutions
First, I show that the first formula does not tautologically imply the second. Consider the truth assignment $$v$$ where $$v(A) = T$$, $$v(B) = F$$, and $$v(C)=F$$. Then $$\overline{v}$$ satisfies the first formula, but does not satisfy the second.

Now, to show that the second formula does not tautologically imply the first, redefine the truth assignment $$v$$ so that $$v(A)=v(B)=v(C)=F$$. Then $$\overline{v}$$ satisfies the second formula, but not the first.

Therefore, neither formula tautologically implies the other
